tutorial/Imp2AsmCorrectness.v
@@ -648,13 +648,21 @@ Section Correctness.
       [alist var value * value] for _Imp_). The differeence is nonetheless mostly
       transparent for the user, except for the use of the more generale [eqit_bind'].
    *)
-  Lemma compile_expr_correct : forall {E} e g_imp g_asm l n,
+  Lemma compile_aexp_correct : forall {E} e g_imp g_asm l n,
       Renv g_imp g_asm ->
       @eutt E _ _ (sim_rel l n)
-            (interp_imp (denote_expr e) g_imp)
-            (interp_asm (denote_list (compile_expr n e)) g_asm l).
+            (interp_imp (denote_aexp e) g_imp)
+            (interp_asm (denote_list (compile_aexp n e)) g_asm l).
   Proof.
     induction e; simpl; intros.
+    - (* Literal case *)
+      (* We reduce both sides to Ret constructs *)
+      tau_steps.
+
+      red; rewrite <-eqit_Ret.
+      (* _Asm_ bind the litteral to [gen_tmp n] while _Imp_ returns it *)
+      apply sim_rel_add; assumption.
+
     - (* Var case *)
       (* We first compute and eliminate taus on both sides. *)
 
@@ -667,14 +675,6 @@ Section Correctness.
       (* On the _Asm_ side, we bind to [gen_tmp n] a lookup to [varOf v] *)
       (* On the _Imp_ side, we return the value of a lookup to [varOf v] *)
       erewrite Renv_find; [| eassumption].
-      apply sim_rel_add; assumption.
-
-    - (* Literal case *)
-      (* We reduce both sides to Ret constructs *)
-      tau_steps.
-
-      red; rewrite <-eqit_Ret.
-      (* _Asm_ bind the litteral to [gen_tmp n] while _Imp_ returns it *)
       apply sim_rel_add; assumption.
 
     (* The three binary operator cases are identical *)
@@ -764,6 +764,13 @@ Section Correctness.
       eapply sim_rel_binary_op; eauto.
   Qed.
 
+  Lemma compile_bexp_correct : forall {E} e g_imp g_asm l n,
+      Renv g_imp g_asm ->
+      @eutt E _ _ (sim_rel l n)
+            (interp_imp (denote_bexp e) g_imp)
+            (interp_asm (denote_list (compile_bexp n e)) g_asm l).
+  Proof.
+ 
   (** Correctness of the assign statement.
       The resulting list of instruction is denoted as
       denoting the expression followed by setting the variable.
